avoid more conversions uint32 -> integer -> nat -> integer

Weidenbach_Book/Array_UInt.thy
@@ -129,4 +129,72 @@ proof -
      nat_of_uint32_code)
 qed
 
+lemma  array_get_hnr_u[sepref_fr_rules]:
+  assumes \<open>CONSTRAINT is_pure A\<close>
+  shows \<open>(uncurry nth_u_code,
+      uncurry (RETURN \<circ>\<circ> op_list_get)) \<in> [pre_list_get]\<^sub>a (array_assn A)\<^sup>k *\<^sub>a uint32_nat_assn\<^sup>k \<rightarrow> A\<close>
+proof -
+  obtain A' where
+    A: \<open>pure A' = A\<close>
+    using assms pure_the_pure by auto
+  then have A': \<open>the_pure A = A'\<close>
+    by auto
+  have [simp]: \<open>the_pure (\<lambda>a c. \<up> ((c, a) \<in> A')) = A'\<close>
+    unfolding pure_def[symmetric] by auto
+  show ?thesis
+    by sepref_to_hoare
+      (sep_auto simp: uint32_nat_rel_def br_def ex_assn_up_eq2 array_assn_def is_array_def
+       hr_comp_def list_rel_pres_length list_rel_update param_nth A' A[symmetric] ent_refl_true
+     list_rel_eq_listrel listrel_iff_nth pure_def nth_u_code_def Array.nth'_def
+     nat_of_uint32_code)
+qed
+
+definition arl_get' :: "'a::heap array_list \<Rightarrow> integer \<Rightarrow> 'a Heap" where
+  [code del]: "arl_get' a i = arl_get a (nat_of_integer i)"
+
+definition arl_get_u :: "'a::heap array_list \<Rightarrow> uint32 \<Rightarrow> 'a Heap" where
+  "arl_get_u \<equiv> \<lambda>a i. arl_get' a (integer_of_uint32 i)"
+
+lemma arl_get'_nth'[code]: \<open>arl_get' = (\<lambda>(a, n). Array.nth' a)\<close>
+  unfolding arl_get_def arl_get'_def Array.nth'_def
+  by (intro ext) auto
+
+lemma arl_get_hnr_u[sepref_fr_rules]:
+  assumes \<open>CONSTRAINT is_pure A\<close>
+  shows \<open>(uncurry arl_get_u, uncurry (RETURN \<circ>\<circ> op_list_get))
+     \<in> [pre_list_get]\<^sub>a (arl_assn A)\<^sup>k *\<^sub>a uint32_nat_assn\<^sup>k \<rightarrow> A\<close>
+proof -
+  obtain A' where
+    A: \<open>pure A' = A\<close>
+    using assms pure_the_pure by auto
+  then have A': \<open>the_pure A = A'\<close>
+    by auto
+  have [simp]: \<open>the_pure (\<lambda>a c. \<up> ((c, a) \<in> A')) = A'\<close>
+    unfolding pure_def[symmetric] by auto
+  show ?thesis
+    by sepref_to_hoare
+      (sep_auto simp: uint32_nat_rel_def br_def ex_assn_up_eq2 array_assn_def is_array_def
+        hr_comp_def list_rel_pres_length list_rel_update param_nth arl_assn_def
+        A' A[symmetric] pure_def arl_get_u_def Array.nth'_def arl_get'_def
+     nat_of_uint32_code[symmetric])
+qed
+
+
+definition heap_array_set' where
+  \<open>heap_array_set' = Array.upd'\<close>
+
+definition heap_array_set'_u where
+  \<open>heap_array_set'_u a i x = heap_array_set' a (integer_of_uint32 i) x \<then> return a\<close>
+
+lemma array_set_hnr_u[sepref_fr_rules]:
+    \<open>CONSTRAINT is_pure A \<Longrightarrow>
+    (uncurry2 heap_array_set'_u, uncurry2 (RETURN \<circ>\<circ>\<circ> op_list_set)) \<in>
+     [pre_list_set]\<^sub>a (array_assn A)\<^sup>d *\<^sub>a uint32_nat_assn\<^sup>k *\<^sub>a A\<^sup>k \<rightarrow> array_assn A\<close>
+  by sepref_to_hoare
+    (sep_auto simp: uint32_nat_rel_def br_def ex_assn_up_eq2 array_assn_def is_array_def
+      hr_comp_def list_rel_pres_length list_rel_update heap_array_set'_u_def
+      heap_array_set'_def Array.upd'_def
+     nat_of_uint32_code[symmetric])
+
+
 end
