Weidenbach_Book/CDCL_Two_Watched_Literals_List_Watched_Init_Trail_Code.thy
@@ -1805,12 +1805,12 @@ sepref_definition SAT_wl_code
   by sepref
 
 
- code_printing constant "shiftl :: nat \<Rightarrow> nat \<Rightarrow> nat" \<rightharpoonup>
+(*  code_printing constant "shiftl :: nat \<Rightarrow> nat \<Rightarrow> nat" \<rightharpoonup>
   (SML) "(nat'_of'_integer(IntInf.<</ (integer'_of'_nat((_)),/ Word.fromInt (integer'_of'_nat((_))))))"
 
 code_printing constant "shiftr :: nat \<Rightarrow> nat \<Rightarrow> nat" \<rightharpoonup>
   (SML) "(nat'_of'_integer(IntInf.~>>/ (integer'_of'_nat((_)),/ Word.fromInt (integer'_of'_nat((_))))))"
-
+ *)
 export_code SAT_wl_code checking SML_imp
 export_code SAT_wl_code
     int_of_integer
